remove C code: alloc_metadata 2/n
trick: avoid vdep \circ vrefine

src/Slabs.fst
@@ -542,160 +542,6 @@ assume val intro_singleton_llist_no_alloc
     SL.v_llist p r' h1 == [SL.get_data (sel r h0)]
   )
 
-//[@@__steel_reduce__]
-//let f
-//  (md_region: array (SL.cell blob){A.length md_region = U32.v metadata_max})
-//  //(md_count_v:U32.t{U32.v md_count_v <= U32.v metadata_max})
-//  (md_count_v: U32.t)
-//  : Pure vprop
-//  (requires U32.v md_count_v <= U32.v metadata_max)
-//  (ensures fun _ -> True)
-//  =
-//  A.varray (A.split_r md_region (u32_to_sz md_count_v))
-//  //(md_count: ref (x:U32.t{U32.v x <= U32.v metadata_max}))
-
-assume val f
-  (p: U32.t -> prop)
-  (v: U32.t)
-  : Pure vprop
-  (requires p v)
-  (ensures fun _ -> True)
-
-//let test_lemma
-//  (md_count: ref U32.t)
-//  (p: U32.t -> prop)
-assume val elim_vdep2 (#opened:SM.inames)
-  (v: vprop)
-  (p: normal (t_of v) -> Tot prop)
-  (f: normal (t_of (vrefine v p)) -> Tot vprop)
-: SteelGhostT (Ghost.erased (normal (t_of (vrefine v p)))) opened
-  (vdep (vrefine v p) f)
-  (fun res -> v `star` f (Ghost.reveal res))
-  //(requires (fun _ -> True))
-  //(ensures (fun h res h' ->
-  //    let fs = h' v in
-  //    let sn : t_of (p (Ghost.reveal res)) = h' (p (Ghost.reveal res)) in
-  //    let x2 = h (vdep v p) in
-  //    Ghost.reveal res == fs /\
-  //    dfst x2 == fs /\
-  //    dsnd x2 == sn
-  //))
-
-#push-options "--z3rlimit 50 --print_implicits --query_stats"
-let test
-  (md_count: ref U32.t)
-  (p: U32.t -> prop)
-  //(f: (v:U32.t{p v}) -> vprop)
-  : SteelT unit
-  //: Steel (SL.t blob)
-  (
-    (vptr md_count `vrefine` p
-      //(fun v -> p v)
-    )
-    `vdep` (f p)//(fun v -> f p v)
-  )
-  (fun r ->
-    (vptr md_count `vrefine` p
-      //(fun v -> p v)
-    )
-    `vdep` (f p)//fun v -> f p v)
-  )
-  =
-  let v_g : G.erased (v:U32.t{p v}) = elim_vdep2
-    (vptr md_count `vrefine` p)
-    (f p) in
-  //slassert (vptr md_count `star` f p v_g);
-  //let v_g2 = G.hide ((G.reveal v_g) <: (v:U32.t{p v})) in
-  //assume (p (G.reveal v_g));
-  //change_slprop_rel
-  //  (f p v_g)
-  //  (f p v_g2)
-  //  (fun x y -> x == y)
-  //  (fun _ -> admit ());
-  //intro_vdep
-  //  (vptr md_count `vrefine` (fun v -> p v))
-  //  (f p v_g)
-  //  (fun v -> f p v);
-  sladmit ();
-  return ()
-
-let a = 42
-
-(*)
-    //(vptr md_count `vrefine`
-    //  (fun v -> U32.v v <= U32.v metadata_max)
-    //) `vdep` (fun v -> f md_region v))
-    //SL.llist (p_empty size_class) r `star`
-    //emp
-    //vptr md_count `vdep` (fun md_count_v ->
-    //vptr md_count `vdep` (fun (md_count_v:U32.t{U32.v md_count_v <= U32.v metadata_max}) ->
-    //  A.varray (A.split_r md_region (u32_to_sz md_count_v))
-    //)
-  //)
-  //(requires fun h0 ->
-  //  let md_count_v
-  //    : U32.t
-  //    = dfst (h0
-  //    (vptr md_count `vdep` (fun v -> f md_region v)))
-  //    //(vptr md_count `vdep`
-  //    //(fun (md_count_v: U32.t{U32.v md_count_v <= U32.v metadata_max}) ->
-  //    //  A.varray (A.split_r md_region (u32_to_sz md_count_v))
-  //    //)))
-  //  in
-  //  U32.v md_count_v < U32.v metadata_max
-  //)
-  //(ensures fun h0 r h1 -> True)
-  =
-  //let x0 = gget (vptr md_count `vdep`
-  //  (fun (md_count_v:U32.t{U32.v md_count_v <= U32.v metadata_max}) ->
-  //    A.varray (A.split_r md_region (u32_to_sz md_count_v)))) in
-  //let x0 = gget (vptr md_count `vdep` (fun v -> f md_region v)) in
-  //sladmit ();
-  //let v0 = G.hide (dfst x0) in
-  //assert (U32.v (G.reveal v0) < U32.v metadata_max);
-  //let v1 : G.erased U32.t = elim_vdep
-  //  (vptr md_count)
-  //  (fun (md_count_v: U32.t{U32.v md_count_v <= U32.v metadata_max}) ->
-  //    A.varray (A.split_r md_region (u32_to_sz md_count_v))) in
-  ////assert (G.reveal v1 == G.reveal v0);
-  //assert (U32.v (G.reveal v1) < U32.v metadata_max);
-  //let v2 : U32.t = read md_count in
-  //assert (v2 == G.reveal v1);
-  //assert (U32.v v2 < U32.v metadata_max);
-  //let md_count_v2 : v:U32.t{U32.v v <= U32.v metadata_max} = read md_count in
-  ////assert (U32.v md_count_v2 = U32.v (sel md_count h0));
-  ////assert (U32.v md_count_v2 < U32.v metadata_max);
-  ////assume (U32.v md_count_v2 < U32.v metadata_max);
-  ////sladmit ();
-  ////let r : SL.t blob = alloc_metadata_aux2 md_count_v size_class slab_region md_bm_region md_region in
-  //write md_count (U32.add md_count_v2 1ul);
-  //let h = get () in
-  //assume (U32.v (sel md_count h) <= U32.v metadata_max);
-  //let md_count_v2 : v:U32.t{U32.v v <= U32.v metadata_max} = read md_count in
-  //sladmit ();
-  return ()
-
-
-let  a = 42
-  //change_slprop_rel
-  //  (A.varray (A.split_r md_region (u32_to_sz md_count_v)))
-  //  (A.varray (A.split_r md_region (u32_to_sz md_count_v2)))
-  //  (fun x y -> x == y)
-  //  (fun _ -> admit ());
-  //intro_vdep
-  //  (vptr md_count)
-  //  (A.varray (A.split_r md_region (u32_to_sz md_count_v2)))
-  //  //  A.varray (A.split_r md_region (u32_to_sz (U32.add md_count_v2 1ul))))
-  //  //(fun md_count_v ->
-  //  (fun (md_count_v: U32.t{U32.v md_count_v <= U32.v metadata_max}) ->
-  //    A.varray (A.split_r md_region (u32_to_sz md_count_v)));
-  //return r
-  return ()
-#pop-options
-
-
-
-
 #push-options "--z3rlimit 30"
 let alloc_metadata_aux2
   (md_count: U32.t{U32.v md_count < U32.v metadata_max})
@@ -703,7 +549,8 @@ let alloc_metadata_aux2
   (slab_region: array U8.t{A.length slab_region = U32.v metadata_max * U32.v page_size})
   (md_bm_region: array U64.t{A.length md_bm_region = U32.v metadata_max * 4})
   (md_region: array (SL.cell blob){A.length md_region = U32.v metadata_max})
-  : Steel (SL.t blob)
+  //: Steel (SL.t blob & (G.erased (v:U32.t{U32.v v = U32.v md_count + 1 /\ U32.v v <= U32.v metadata_max})))
+  : Steel (SL.t blob & (G.erased U32.t))
   (
     A.varray (A.split_r slab_region (u32_to_sz (U32.mul md_count page_size))) `star`
     A.varray (A.split_r md_bm_region (u32_to_sz (U32.mul md_count 4ul))) `star`
@@ -712,14 +559,16 @@ let alloc_metadata_aux2
   //TODO: add a refinement over a md_count ref, discussion with Aymeric
   ////`star` vptr md_count)
   (fun r ->
-    SL.llist (p_empty size_class) r `star`
+    SL.llist (p_empty size_class) (fst r) `star`
     A.varray (A.split_r slab_region (u32_to_sz (U32.mul (U32.add md_count 1ul) page_size))) `star`
     A.varray (A.split_r md_bm_region (u32_to_sz (U32.mul (U32.add md_count 1ul) 4ul))) `star`
     A.varray (A.split_r md_region (u32_to_sz (U32.add md_count 1ul)))
   )
   (requires fun h0 -> True)
   (ensures fun h0 r h1 ->
-    L.length (SL.v_llist (p_empty size_class) r h1) = 1
+    L.length (SL.v_llist (p_empty size_class) (fst r) h1) = 1 /\
+    G.reveal (snd r) = U32.add md_count 1ul /\
+    U32.v (G.reveal (snd r)) <= U32.v metadata_max
   )
   =
   let b : blob = alloc_metadata_aux md_count size_class slab_region md_bm_region md_region in
@@ -736,7 +585,7 @@ let alloc_metadata_aux2
   let b_cell = SL.mk_cell null b in
   write r b_cell;
   let r = intro_singleton_llist_no_alloc (p_empty size_class) r b in
-  return r
+  return (r, G.hide (U32.add md_count 1ul))
 #pop-options
 
 #push-options "--z3rlimit 100"
@@ -745,130 +594,70 @@ let alloc_metadata
   (slab_region: array U8.t{A.length slab_region = U32.v metadata_max * U32.v page_size})
   (md_bm_region: array U64.t{A.length md_bm_region = U32.v metadata_max * 4})
   (md_region: array (SL.cell blob){A.length md_region = U32.v metadata_max})
-  //(md_count: ref (x:U32.t{U32.v x <= U32.v metadata_max}))
   (md_count: ref U32.t)
-  : Steel unit
-  //: Steel (SL.t blob)
+  (md_count_v: G.erased (v:U32.t{U32.v v < U32.v metadata_max}))
+  //: Steel (SL.t blob & (G.erased (v:U32.t{U32.v v = U32.v md_count_v + 1 /\ U32.v v <= U32.v metadata_max})))
+  : Steel ((SL.t blob) & (G.erased U32.t))
   (
-    vptr md_count `vdep` (fun (md_count_v:U32.t{U32.v md_count_v <= U32.v metadata_max}) ->
-    //vptr md_count `vdep` (fun (md_count_v: U32.t{U32.v md_count_v < U32.v metadata_max}) ->
-      A.varray (A.split_r slab_region (u32_to_sz (U32.mul md_count_v page_size))) `star`
-      A.varray (A.split_r md_bm_region (u32_to_sz (U32.mul md_count_v 4ul))) `star`
-      A.varray (A.split_r md_region (u32_to_sz md_count_v))
-    )
+    vptr md_count `star`
+    A.varray (A.split_r slab_region (u32_to_sz (U32.mul (G.reveal md_count_v) page_size))) `star`
+    A.varray (A.split_r md_bm_region (u32_to_sz (U32.mul (G.reveal md_count_v) 4ul))) `star`
+    A.varray (A.split_r md_region (u32_to_sz (G.reveal md_count_v)))
   )
-  //TODO: add a refinement over a md_count ref, discussion with Aymeric
-  ////`star` vptr md_count)
   (fun r ->
-    //SL.llist (p_empty size_class) r `star`
-    //emp
-    //vptr md_count `vdep` (fun md_count_v ->
-    vptr md_count `vdep` (fun (md_count_v:U32.t{U32.v md_count_v <= U32.v metadata_max}) ->
-      A.varray (A.split_r slab_region (u32_to_sz (U32.mul md_count_v page_size))) `star`
-      A.varray (A.split_r md_bm_region (u32_to_sz (U32.mul md_count_v 4ul))) `star`
-      A.varray (A.split_r md_region (u32_to_sz md_count_v))
-    )
+    vptr md_count `star`
+    SL.llist (p_empty size_class) (fst r) `star`
+    A.varray (A.split_r slab_region (u32_to_sz (U32.mul (U32.add (G.reveal md_count_v) 1ul) page_size))) `star`
+    A.varray (A.split_r md_bm_region (u32_to_sz (U32.mul (U32.add (G.reveal md_count_v) 1ul) 4ul))) `star`
+    A.varray (A.split_r md_region (u32_to_sz (U32.add (G.reveal md_count_v) 1ul)))
   )
-  (requires fun h0 ->
-    let md_count_v
-      : U32.t
-      = dfst (h0
-      (vptr md_count `vdep`
-      (fun (md_count_v: U32.t{U32.v md_count_v <= U32.v metadata_max}) ->
-        A.varray (A.split_r slab_region (u32_to_sz (U32.mul md_count_v page_size))) `star`
-        A.varray (A.split_r md_bm_region (u32_to_sz (U32.mul md_count_v 4ul))) `star`
-        A.varray (A.split_r md_region (u32_to_sz md_count_v))
-      )))
-    in
-    U32.v md_count_v < U32.v metadata_max
-  )
-  (ensures fun h0 r h1 -> True)
-  //(ensures fun h0 r h1 ->
-  //  let md_count_v
-  //    : U32.t
-  //    = dfst (h1
-  //    (vptr md_count `vdep`
-  //    (fun (md_count_v: U32.t{U32.v md_count_v <= U32.v metadata_max}) ->
-  //      A.varray (A.split_r slab_region (u32_to_sz (U32.mul md_count_v page_size))) `star`
-  //      A.varray (A.split_r md_bm_region (u32_to_sz (U32.mul md_count_v 4ul))) `star`
-  //      A.varray (A.split_r md_region (u32_to_sz md_count_v))
-  //    )))
-  //  in
-  //  U32.v md_count_v <= U32.v metadata_max)
-
-
-  //  let md_count_v0
-  //    : U32.t
-  //    = dfst (h0
-  //    (vptr md_count `vdep`
-  //    (fun md_count_v ->
-  //      A.varray (A.split_r slab_region (u32_to_sz (U32.mul md_count_v page_size))) `star`
-  //      A.varray (A.split_r md_bm_region (u32_to_sz (U32.mul md_count_v 4ul))) `star`
-  //      A.varray (A.split_r md_region (u32_to_sz md_count_v))
-  //    ))) in
-  //  let md_count_v1
-  //    : U32.t
-  //    = dfst (h1
-  //    (vptr md_count `vdep`
-  //    (fun md_count_v ->
-  //      A.varray (A.split_r slab_region (u32_to_sz (U32.mul md_count_v page_size))) `star`
-  //      A.varray (A.split_r md_bm_region (u32_to_sz (U32.mul md_count_v 4ul))) `star`
-  //      A.varray (A.split_r md_region (u32_to_sz md_count_v))
-  //    ))) in
-  //  md_count_v0 = md_count_v1
-
-
-
-  ////  //sel md_count h1 = sel md_count h0
-  ////  //L.length (SL.v_llist (p_empty size_class) r h1) = 1
+  //  SL.llist (p_empty size_class) (fst r) `star`
+    //A.varray (A.split_r slab_region (u32_to_sz (U32.mul (G.reveal (snd r)) page_size))) `star`
+    //A.varray (A.split_r md_bm_region (u32_to_sz (U32.mul (G.reveal (snd r)) 4ul))) `star`
+    //A.varray (A.split_r md_region (u32_to_sz (G.reveal (snd r)))))
   //)
+  (requires fun h0 ->
+    sel md_count h0 = G.reveal md_count_v
+  )
+  (ensures fun h0 r h1 ->
+  //  L.length (SL.v_llist (p_empty size_class) (fst r) h1) = 1 /\
+    sel md_count h0 = G.reveal md_count_v /\
+    sel md_count h1 = U32.add (sel md_count h0) 1ul /\
+    sel md_count h1 = G.reveal (snd r)
+  )
   =
-  admit ();
-  let md_count_v = elim_vdep
-    (vptr md_count)
-    //(fun md_count_v ->
-    (fun (md_count_v: U32.t{U32.v md_count_v <= U32.v metadata_max}) ->
-      A.varray (A.split_r slab_region (u32_to_sz (U32.mul md_count_v page_size))) `star`
-      A.varray (A.split_r md_bm_region (u32_to_sz (U32.mul md_count_v 4ul))) `star`
-      A.varray (A.split_r md_region (u32_to_sz md_count_v))) in
-
-  let h0 = get () in
-  assume (U32.v (sel md_count h0) < U32.v metadata_max);
-  //let md_count_v2 = read md_count in
-  let md_count_v2 : v:U32.t{U32.v v <= U32.v metadata_max} = read md_count in
-  //assert (U32.v md_count_v2 = U32.v (sel md_count h0));
-  //assert (U32.v md_count_v2 < U32.v metadata_max);
-  //assume (U32.v md_count_v2 < U32.v metadata_max);
-  //sladmit ();
-  //let r : SL.t blob = alloc_metadata_aux2 md_count_v size_class slab_region md_bm_region md_region in
-  write md_count (U32.add md_count_v2 1ul);
-  let h = get () in
-  assume (U32.v (sel md_count h) <= U32.v metadata_max);
-  let md_count_v2 : v:U32.t{U32.v v <= U32.v metadata_max} = read md_count in
+  let md_count_v0 = read md_count in
+  assert (md_count_v0 == G.reveal md_count_v);
+  assert (U32.v md_count_v0 < U32.v metadata_max);
   change_slprop_rel
-    (A.varray (A.split_r slab_region (u32_to_sz (U32.mul md_count_v page_size))) `star`
-      A.varray (A.split_r md_bm_region (u32_to_sz (U32.mul md_count_v 4ul))) `star`
-      A.varray (A.split_r md_region (u32_to_sz md_count_v)))
-    (A.varray (A.split_r slab_region (u32_to_sz (U32.mul md_count_v2 page_size))) `star`
-      A.varray (A.split_r md_bm_region (u32_to_sz (U32.mul md_count_v2 4ul))) `star`
-      A.varray (A.split_r md_region (u32_to_sz md_count_v2)))
+    (A.varray (A.split_r slab_region (u32_to_sz (U32.mul (G.reveal md_count_v) page_size))) `star`
+    A.varray (A.split_r md_bm_region (u32_to_sz (U32.mul (G.reveal md_count_v) 4ul))) `star`
+    A.varray (A.split_r md_region (u32_to_sz (G.reveal md_count_v))))
+    (A.varray (A.split_r slab_region (u32_to_sz (U32.mul md_count_v0 page_size))) `star`
+    A.varray (A.split_r md_bm_region (u32_to_sz (U32.mul md_count_v0 4ul))) `star`
+    A.varray (A.split_r md_region (u32_to_sz md_count_v0)))
     (fun x y -> x == y)
     (fun _ -> admit ());
-  intro_vdep
-    (vptr md_count)
-    (A.varray (A.split_r slab_region (u32_to_sz (U32.mul md_count_v2 page_size))) `star`
-      A.varray (A.split_r md_bm_region (u32_to_sz (U32.mul md_count_v2 4ul))) `star`
-      A.varray (A.split_r md_region (u32_to_sz md_count_v2)))
-    //(A.varray (A.split_r slab_region (u32_to_sz (U32.mul (U32.add md_count_v2 1ul) page_size))) `star`
-    //  A.varray (A.split_r md_bm_region (u32_to_sz (U32.mul (U32.add md_count_v2 1ul) 4ul))) `star`
-    //  A.varray (A.split_r md_region (u32_to_sz (U32.add md_count_v2 1ul))))
-    //(fun md_count_v ->
-    (fun (md_count_v: U32.t{U32.v md_count_v <= U32.v metadata_max}) ->
-      A.varray (A.split_r slab_region (u32_to_sz (U32.mul md_count_v page_size))) `star`
-      A.varray (A.split_r md_bm_region (u32_to_sz (U32.mul md_count_v 4ul))) `star`
-      A.varray (A.split_r md_region (u32_to_sz md_count_v)));
-  //return r
-  return ()
+  let r = alloc_metadata_aux2 md_count_v0 size_class slab_region md_bm_region md_region in
+  write md_count (U32.add md_count_v0 1ul);
+  let md_count_v1 = read md_count in
+  assert (U32.v md_count_v1 = U32.v (G.reveal snd r));
+  //admit ();
+  //assert (md_count_v1 = U32.add md_count_v0 1ul);
+  //assert (U32.v md_count_v0 <= U32.v metadata_max);
+
+  change_slprop_rel
+    (A.varray (A.split_r slab_region (u32_to_sz (U32.mul (U32.add md_count_v0 1ul) page_size))) `star`
+    A.varray (A.split_r md_bm_region (u32_to_sz (U32.mul (U32.add md_count_v0 1ul) 4ul))) `star`
+    A.varray (A.split_r md_region (u32_to_sz (U32.add md_count_v0 1ul))))
+    (A.varray (A.split_r slab_region (u32_to_sz (U32.mul (U32.add (G.reveal md_count_v) 1ul) page_size))) `star`
+    A.varray (A.split_r md_bm_region (u32_to_sz (U32.mul (U32.add (G.reveal md_count_v) 1ul) 4ul))) `star`
+    A.varray (A.split_r md_region (u32_to_sz (U32.add (G.reveal md_count_v) 1ul))))
+    (fun x y -> x == y)
+    (fun _ -> admit ());
+  //sladmit ();
+  return r
+  //return (fst r, G.hide (md_count_v1))
 #pop-options
 
 
